EffectSSA/Types/Context.lean
@@ -1,4 +1,5 @@
 import EffectSSA.Types.Context.Basic
 import EffectSSA.Types.Context.Lemmas
 import EffectSSA.Types.Context.TVar
+import EffectSSA.Types.Context.TVarList
 import EffectSSA.Types.Context.Hom
