EffectSSA/Types/Context/TVarList.lean
@@ -1,0 +1,122 @@
+import EffectSSA.Types.Context.Basic
+import EffectSSA.Types.Context.Lemmas
+import EffectSSA.Types.Context.TVar
+import EffectSSA.Types.Context.Hom
+
+/-!
+# Intrinsically Well-typed List of Variables
+
+`TVarList Γ Δ` is essentially a list of `TVar`s in the same context `Γ`, but
+with different types, as specified by the output context `Δ`.
+This can be seen as a context homomorphism `Δ.Hom Γ` (note the reversal of the
+contexts), as shown by `TVarList.asHom`.
+-/
+namespace EffectSSA
+variable {τ}
+
+/-
+TODO: If `TVarList` is isomorphic to a context isomorphism, do we really need both?
+
+One argument is that they have different tradeoffs: the `TVarList` materializes
+the mapping as a list, making it computationally nicer (but we do really care
+about this?), whereas the `Hom` definition is easier to compose with an arbitrary
+function without needing extra API (although this API certainly could be written
+for TVarList as well).
+
+In particular, the TVarList is a natural evolution of specifying return variables
+of a program as a list of variables, but `Hom` makes sense for specifying an
+arbitrary substitution. Let's see how these things actually get used before
+unifying them.
+-/
+
+/--
+`vs : TVarList Γ Δ` is a list of variables,
+such that `vs[i]` is assigned the respective type `Δ[i]` in `Γ`.
+-/
+structure TVarList (Γ : Context τ) (Δ : Context τ) where
+  toList : List Var
+  length_eq : toList.length = Δ.size := by grind
+  wt : ∀ (i : Fin Δ.size), Γ[toList[i]]? = Δ[Var.ofNat i]? := by grind
+
+
+/-!
+## Grind Attributes
+--------------------------------------------------------------------------------
+-/
+
+grind_pattern TVar.wt => TVar.toVar self
+attribute [grind =] TVarList.wt
+
+grind_pattern TVarList.length_eq => TVarList.toList self
+
+/-!
+## Definitions
+--------------------------------------------------------------------------------
+-/
+namespace TVarList
+
+@[grind] abbrev length (vs : TVarList Γ ts) : Nat := vs.toList.length
+
+/--
+A `TVarList Γ Δ` can be seen as a context homomorphism `Δ.Hom Γ`.
+
+This works because a list `vs : TVarList Γ Δ` has exactly as many elements as
+variables in `Δ`, and the element of `vs` that corresponds to some `TVar Δ t` is
+a `TVar Γ t`.
+Thus, the induced morphism just looks up the corresponding entry in the list.
+-/
+def asHom (vs : TVarList Γ Δ) : Δ.Hom Γ where
+  raw v := vs.toList[v.toNat]?.getD v
+  ty_eq := by
+    intro v t (hv : _ = some _)
+    have := vs.wt ⟨v.toNat, by
+      change Δ.toList[v.toNat]? = _ at hv
+      grind⟩
+    grind
+
+/--
+`vs.get v` returns the variable (in `Γ`) that the list `vs : TVarList Γ Δ`
+associates with a variable `v` in `Δ`.
+
+This is an alias for `vs.asHom.apply`.
+-/
+abbrev get (vs : TVarList Γ Δ) : TVar Δ t → TVar Γ t :=
+  vs.asHom.apply
+
+/--
+Map a function into a non-dependent type `α` over a TVarList, yielding a regular
+(homogeneous) list.
+
+Note that the function is _only_ applied to variables which are live, according
+to `Δ`, any stale variables are ignored.
+-/
+def map (f : ∀ {t}, TVar Γ t → α) (vs : TVarList Γ Δ) : List α :=
+  Δ.toList.zipIdx.attach.map fun ⟨⟨t, i⟩, h⟩ =>
+    let v : TVar Δ t := ⟨.ofNat i, by
+      show Δ.toList[i]? = some t
+      grind⟩
+    f (vs.get v)
+
+/-!
+## Lemmas
+--------------------------------------------------------------------------------
+-/
+section Lemmas
+variable {ts} (f : ∀ {t}, TVar Γ t → α) (vs : TVarList Γ Δ)
+
+@[simp] theorem length_map : (vs.map f).length = Δ.size := by
+  simp [map]
+
+@[grind =]
+theorem getElem?_map (i : Nat) :
+    (vs.map @f)[i]? =
+      let i := Var.ofNat i
+      if hi : i.InBounds Δ then
+        some <| @f Δ[i] <| vs.get ⟨i, by grind⟩
+      else
+        none := by
+  by_cases hi : (Var.ofNat i).InBounds Δ
+  · grind [map]
+  · simp [hi]; grind
+
+end Lemmas
